sugar

src/Example.Check.Simple.fst
@@ -1,14 +1,15 @@
 (* Checking a simple example *)
 module Example.Check.Simple
 
-open Pipit.Exp.Base
+module Exp = Pipit.Exp.Base
 
-open Pipit.System.Base
-open Pipit.System.Ind
-open Pipit.System.Exp
+// open Pipit.System.Base
+// open Pipit.System.Ind
+// open Pipit.System.Exp
 
 module T = FStar.Tactics
-module Sugar = Pipit.Sugar
+module Sugar = Pipit.SugarX3
+open Sugar
 
 let tac_nbe (): T.Tac unit = T.norm [primops; iota; delta; zeta; nbe]
 
@@ -19,27 +20,41 @@ let tac_nbe (): T.Tac unit = T.norm [primops; iota; delta; zeta; nbe]
        (if p then 1 else 0)
 *)
 inline_for_extraction
-let count_when (p: exp) =
- let open Sugar in
- mu' (
-   let count = XVar 0 in
-   let p' = lift' p in
-
-   (z0 --> pre count) +^ (ite p' z1 z0))
+let count_when (p: stream bool): Stream (stream int) =
+ rec' (fun count ->
+   fby 0 count +^ (ite p z1 z0))
 
 (* forall e. count_when false <= count_when e <= count_when true *)
-let count_when_prop =
-  let open Sugar in
-  system_of_exp (
-    let' (count_when ff) (
-      let' (count_when x0) (
-        let' (count_when tt) (
-          let count_when_false = x2 in
-          let count_when_e = x1 in
-          let count_when_true = x0 in
-          count_when_false <=^ count_when_e /\ count_when_e <=^ count_when_true))))
-    1
+let count_when_prop (e: stream bool): Stream (stream unit) =
+  let' (count_when ff) (fun count_when_false ->
+  let' (count_when e) (fun count_when_e ->
+  let' (count_when tt) (fun count_when_true ->
+  check' "count_when false <= count_when e" (count_when_false <=^ count_when_e) (
+  check' "cwe<=cwt" (count_when_e <=^ count_when_true) (
+  pure ())))))
 
-let count_when_prop_prove (): Lemma (ensures induct1' count_when_prop) =
-  assert (base_case' count_when_prop) by tac_nbe ();
-  assert (step_case' count_when_prop) by tac_nbe ()
+let run (e: unit -> Stream 'a) : 'a =
+  let (a, _) = reify (e ()) { fresh = 0 } in
+  a
+
+
+let sdf (): Stream unit =
+  let xe = run (fun _ -> count_when_prop tt) in
+  assert (xe == (pure ())) by (T.norm [primops; iota; delta]; T.norm [nbe]; T.dump "")
+  // by (tac_nbe (); T.dump "")
+
+
+//   let open Sugar in
+//   system_of_exp (
+//     let' (count_when ff) (
+//       let' (count_when x0) (
+//         let' (count_when tt) (
+//           let count_when_false = x2 in
+//           let count_when_e = x1 in
+//           let count_when_true = x0 in
+//           count_when_false <=^ count_when_e /\ count_when_e <=^ count_when_true))))
+//     1
+
+// let count_when_prop_prove (): Lemma (ensures induct1' count_when_prop) =
+//   assert (base_case' count_when_prop) by tac_nbe ();
+//   assert (step_case' count_when_prop) by tac_nbe ()
