src/Pipit.Exp.Base.fst
@@ -11,7 +11,7 @@ type exp (c: C.context) 'a =
   // bound variable (de Bruijn index)
   | XBVar  : (i: C.index { C.opt_index c i == Some 'a }) -> exp c 'a
   // free variables
-  | XVar   : (x: C.var { C.opt_var c x == Some 'a }) -> exp c 'a
+  | XVar   : (x: C.var 'a) -> exp c 'a
   // f(e,...)
   | XApp   : exp c ('b -> 'a) -> exp c 'b -> exp c 'a
   // v fby e
@@ -19,63 +19,60 @@ type exp (c: C.context) 'a =
   // e -> e'
   | XThen  : exp c 'a -> exp c 'a -> exp c 'a
   // µx. e[x]
-  | XMu    : exp (C.bind_index1 c 'a) 'a -> exp c 'a
+  | XMu    : exp ('a :: c) 'a -> exp c 'a
   // let x = e in e[x]
-  | XLet   : (b: Type) -> exp c b -> exp (C.bind_index1 c b) 'a -> exp c 'a
+  | XLet   : (b: Type) -> exp c b -> exp (b :: c) 'a -> exp c 'a
 
   // Proof terms
   // Contracts for hiding implementation:
   //   (λx. { assumes } body { λr. guarantees })(arg)
   | XContract:
-           (assumes: exp (C.from_indices ['b]) xprop) ->
-           (guarantees: exp (C.from_indices ['a; 'b]) xprop) ->
-           (body: exp (C.from_indices ['b]) 'a) ->
+           (assumes: exp ['b] xprop) ->
+           (guarantees: exp ['a; 'b] xprop) ->
+           (body: exp ['b] 'a) ->
            (arg: exp c 'b) ->
            exp c 'a
   // check "" e in e
   | XCheck : string -> exp c xprop -> exp c 'a -> exp c 'a
 
-let exp' (c: C.closed) 'a = exp c 'a
-
-let rec open1' (#c: C.context) (e: exp c 'a) (x: C.var { C.fresh c x }) (n: C.index { C.has_index c n }): Tot (exp (C.open1' c x n) 'a) (decreases e) =
+let rec open1' (#c: C.context) (e: exp c 'a) (n: C.index { C.has_index c n }) (x: C.var (C.get_index c n)): Tot (exp (C.open1' c n) 'a) (decreases e) =
   match e with
   | XVal v -> XVal v
   | XBVar i ->
     if i = n
     then
-      (C.open_contains_opt_var_lemma c x n;
-      XVar x)
+      XVar x
     else
-      (C.open_preserves_opt_index_lemma c x n i;
+      (C.open_preserves_opt_index_lemma c n i;
       XBVar (C.index_drop i n 1))
   | XVar x' ->
-    C.open_preserves_opt_var_lemma c x n x';
     XVar x'
-  | XApp f e -> XApp (open1' f x n) (open1' e x n)
-  | XFby v e -> XFby v (open1' e x n)
-  | XThen e1 e2 -> XThen (open1' e1 x n) (open1' e2 x n)
-  | XMu e -> XMu (open1' e x (n + 1))
+  | XApp f e -> XApp (open1' f n x) (open1' e n x)
+  | XFby v e -> XFby v (open1' e n x)
+  | XThen e1 e2 -> XThen (open1' e1 n x) (open1' e2 n x)
+  | XMu e -> XMu (open1' e (n + 1) x)
   | XLet b e1 e2 ->
-    let e1' = open1' e1 x n in
-    let e2' = open1' e2 x (n + 1) in
+    let e1' = open1' e1 n x in
+    let e2' = open1' e2 (n + 1) x in
     XLet b e1' e2'
   | XContract a g b arg  ->
-    XContract a g b (open1' arg x n)
-  | XCheck name e1 e2 -> XCheck name (open1' e1 x n) (open1' e2 x n)
+    XContract a g b (open1' arg n x)
+  | XCheck name e1 e2 -> XCheck name (open1' e1 n x) (open1' e2 n x)
 
-let rec close1' (#c: C.context) (e: exp c 'a) (x: C.var { C.has_var c x }) (n: C.index { n <= List.Tot.length c.bound }): Tot (exp (C.close1' c x n) 'a) (decreases e) =
+let rec close1' (#c: C.context) (e: exp c 'a) (x: C.var 'b) (n: C.index { n <= List.Tot.length c }): Tot (exp (C.close1' c 'b n) 'a) (decreases e) =
   match e with
   | XVal v -> XVal v
   | XBVar i ->
-    C.close_preserves_opt_index_lemma c x n i;
+    C.close_preserves_opt_index_lemma c 'b n i;
     XBVar (C.index_lift i n 1)
   | XVar x' ->
-    if x = x'
+    if C.Var?.v x = C.Var?.v x'
     then
-      (C.close_opt_var_contains_lemma c x n;
+      (C.cheat_variables_assume_global x x';
+      C.close_contains_lemma c 'b n;
       XBVar n)
     else
-      (C.close_preserves_opt_var_lemma c x n x';
+      (// C.close_preserves_opt_var_lemma c x n x';
       XVar x')
   | XApp f e -> XApp (close1' f x n) (close1' e x n)
   | XFby v e -> XFby v (close1' e x n)
@@ -85,14 +82,15 @@ let rec close1' (#c: C.context) (e: exp c 'a) (x: C.var { C.has_var c x }) (n: C
   | XContract a g b arg -> XContract a g b (close1' arg x n)
   | XCheck name e1 e2 -> XCheck name (close1' e1 x n) (close1' e2 x n)
 
-let open1 (e: exp 'c 'a { C.has_index 'c 0 }) x = open1' e x 0
+let open1 (e: exp 'c 'a { C.has_index 'c 0 }) x = open1' e 0 x
 let close1 (e: exp 'c 'a) x = close1' e x 0
 
-let rec lift1' (#c: C.context) (e: exp c 'a) (n: C.index { n <= List.Tot.length c.bound }) (t: Type): Tot (exp (C.bind_index1' c n t) 'a) (decreases e) =
+let rec lift1' (#c: C.context) (e: exp c 'a) (n: C.index { n <= List.Tot.length c }) (t: Type): Tot (exp (C.lift1 c n t) 'a) (decreases e) =
   match e with
   | XVal v -> XVal v
   | XBVar i ->
-    C.bind_index_preserves_opt_index_lemma c n i t;
+    // C.bind_index_preserves_opt_index_lemma c n i t;
+    C.close_preserves_opt_index_lemma c t n i;
     XBVar (C.index_lift i n 1)
   | XVar x' ->
     XVar x'
@@ -100,57 +98,57 @@ let rec lift1' (#c: C.context) (e: exp c 'a) (n: C.index { n <= List.Tot.length 
   | XFby v e -> XFby v (lift1' e n t)
   | XThen e1 e2 -> XThen (lift1' e1 n t) (lift1' e2 n t)
   | XMu e1 ->
-    let e1': exp (C.bind_index1' (C.bind_index1 c 'a) (n + 1) t) 'a = lift1' e1 (n + 1) t in
-    let e1'': exp (C.bind_index1 (C.bind_index1' c n t) 'a) 'a = e1' in
+    let e1': exp (C.lift1 (C.lift1 c 0 'a) (n + 1) t) 'a = lift1' e1 (n + 1) t in
+    let e1'': exp (C.lift1 (C.lift1 c n t) 0 'a) 'a = e1' in
     XMu e1''
   | XLet b e1 e2 -> XLet b (lift1' e1 n t) (lift1' e2 (n + 1) t)
   | XContract a g b arg ->
     XContract a g b (lift1' arg n t)
   | XCheck name e1 e2 -> XCheck name (lift1' e1 n t) (lift1' e2 n t)
 
-let lift1 (#c: C.context) (e: exp c 'a) (t: Type): exp (C.bind_index1 c t) 'a =
+let lift1 (#c: C.context) (e: exp c 'a) (t: Type): exp (C.lift1 c 0 t) 'a =
   lift1' e 0 t
 
-let rec subst_index1' (#c: C.context) (e: exp c 'a) (i: C.index { C.has_index c i }) (payload: exp (C.drop_index1 c i) (C.get_index c i)): Tot (exp (C.drop_index1 c i) 'a) (decreases e) =
+let rec subst_index1' (#c: C.context) (e: exp c 'a) (i: C.index { C.has_index c i }) (payload: exp (C.drop1 c i) (C.get_index c i)): Tot (exp (C.drop1 c i) 'a) (decreases e) =
   match e with
   | XVal v -> XVal v
   | XBVar i' ->
     if i' = i
     then payload
     else
-      (C.drop_index_preserves_opt_index_lemma c i i';
+      (C.open_preserves_opt_index_lemma c i i';
       XBVar (C.index_drop i' i 1))
   | XVar x' -> XVar x'
   | XApp f e -> XApp (subst_index1' f i payload) (subst_index1' e i payload)
   | XFby v e -> XFby v (subst_index1' e i payload)
   | XThen e1 e2 -> XThen (subst_index1' e1 i payload) (subst_index1' e2 i payload)
   | XMu e1 ->
-    let e1': exp (C.drop_index1 (C.bind_index1 c 'a) (i + 1)) 'a = subst_index1' e1 (i + 1) (lift1 payload 'a) in
-    let e1'': exp (C.bind_index1 (C.drop_index1 c i) 'a) 'a = e1' in
+    let e1': exp (C.drop1 (C.lift1 c 0 'a) (i + 1)) 'a = subst_index1' e1 (i + 1) (lift1 payload 'a) in
+    let e1'': exp (C.lift1 (C.drop1 c i) 0 'a) 'a = e1' in
     XMu e1''
   | XLet b e1 e2 -> XLet b (subst_index1' e1 i payload) (subst_index1' e2 (i + 1) (lift1 payload b))
   | XContract a g b arg ->
     XContract a g b (subst_index1' arg i payload)
   | XCheck name e1 e2 -> XCheck name (subst_index1' e1 i payload) (subst_index1' e2 i payload)
 
-let subst_index1 (#c: C.context { C.has_index c 0 }) (e: exp c 'a) (payload: exp (C.drop_index1 c 0) (C.get_index c 0)): Tot (exp (C.drop_index1 c 0) 'a) (decreases e) =
+let subst_index1 (#c: C.context { C.has_index c 0 }) (e: exp c 'a) (payload: exp (C.drop1 c 0) (C.get_index c 0)): Tot (exp (C.drop1 c 0) 'a) (decreases e) =
   subst_index1' e 0 payload
 
-let rec weaken_closed (#c c': C.closed) (e: exp c 'a): Tot (exp (C.append_closed c c') 'a) (decreases e) =
+let rec weaken (#c c': C.context) (e: exp c 'a): Tot (exp (C.append c c') 'a) (decreases e) =
   match e with
   | XVal v -> XVal v
   | XBVar i' ->
     C.append_preserves_opt_index_lemma c c' i';
     XBVar i'
   | XVar x' -> XVar x'
-  | XApp f e -> XApp (weaken_closed c' f) (weaken_closed c' e)
-  | XFby v e -> XFby v (weaken_closed c' e)
-  | XThen e1 e2 -> XThen (weaken_closed c' e1) (weaken_closed c' e2)
+  | XApp f e -> XApp (weaken c' f) (weaken c' e)
+  | XFby v e -> XFby v (weaken c' e)
+  | XThen e1 e2 -> XThen (weaken c' e1) (weaken c' e2)
   | XMu e1 ->
-    let e1': exp (C.append_closed (C.bind_index1 c 'a) c') 'a = weaken_closed c' e1 in
-    let e1'': exp (C.bind_index1 (C.append_closed c c') 'a) 'a = e1' in
+    let e1': exp (C.append (C.lift1 c 0 'a) c') 'a = weaken c' e1 in
+    let e1'': exp (C.lift1 (C.append c c') 0 'a) 'a = e1' in
     XMu e1''
-  | XLet b e1 e2 -> XLet b (weaken_closed c' e1) (weaken_closed c' e2)
+  | XLet b e1 e2 -> XLet b (weaken c' e1) (weaken c' e2)
   | XContract a g b arg ->
-    XContract a g b (weaken_closed c' arg)
-  | XCheck name e1 e2 -> XCheck name (weaken_closed c' e1) (weaken_closed c' e2)
+    XContract a g b (weaken c' arg)
+  | XCheck name e1 e2 -> XCheck name (weaken c' e1) (weaken c' e2)
